first pass at AtomicPair
still using symbolic execution, which assumes no crashes in a few places

let's see if it's doable without [prog_spec] style specs..

src/Disk/Sectors.v
@@ -8,11 +8,20 @@ Definition addr := nat.
 (* We introduce this definition to make the large constant opaque, for
 performance reasons. *)
 Definition blockbytes := 1024.
-Opaque blockbytes.
 
 Definition block := bytes blockbytes.
-Definition block0 : block := bytes0 blockbytes.
+Definition block0 : block := bytes0 _.
+Definition block1 : block := bytes1 _.
+
+Theorem block0_block1_differ : block0 <> block1.
+Proof.
+  apply bytes_differ.
+Qed.
+
+Hint Resolve block0_block1_differ.
 
 (* To deal with Coq v8.6 not having https://github.com/coq/coq/pull/876 yet *)
 Local Ltac omega_orig := omega.
 Ltac omega := unfold addr in *; omega_orig.
+
+Opaque blockbytes.
