src/AtomicPair/AtomicPairAPI.v
@@ -1,0 +1,31 @@
+Require Import POCS.
+
+Module AtomicPair.
+
+  Inductive Op : Type -> Type :=
+  | Get : Op (block*block)
+  | Put (p : block*block) : Op unit.
+
+  Definition State : Type := block*block.
+
+  (* help out type inference *)
+  Implicit Type (state:State).
+
+  Inductive step : forall `(op: Op T), Semantics State T :=
+  | step_get : forall s r,
+      s = r ->
+      step (Get) s r s
+  | step_put : forall s v,
+      step (Put v) s tt v.
+
+  Definition crash_relation state state' := state' = state.
+  Definition inited state := True.
+
+  Definition API : InterfaceAPI Op State :=
+    {|
+      op_sem := @step;
+      crash_effect := crash_relation;
+      init_sem := inited;
+    |}.
+
+End AtomicPair.
