src/AtomicPair/AtomicPairImpl.v
@@ -1,0 +1,138 @@
+Require Import POCS.
+Require Import AtomicPair.AtomicPairAPI.
+Require Import OneDisk.OneDiskAPI.
+
+Import OneDisk.
+Import AtomicPair.
+
+Module AtomicPair.
+
+  Section Implementation.
+
+    Variable (d : Interface OneDisk.API).
+
+    Definition get : prog (block*block) :=
+      ptr <- Prim d (Read 0);
+      if ptr == block0 then
+        a <- Prim d (Read 1);
+        b <- Prim d (Read 2);
+        Ret (a, b)
+      else
+        a <- Prim d (Read 3);
+        b <- Prim d (Read 4);
+        Ret (a, b).
+
+    Definition put (p : block*block) : prog unit :=
+      ptr <- Prim d (Read 0);
+      if ptr == block0 then
+        _ <- Prim d (Write 3 (fst p));
+        _ <- Prim d (Write 4 (snd p));
+        _ <- Prim d (Write 0 block1);
+        Ret tt
+      else
+        _ <- Prim d (Write 1 (fst p));
+        _ <- Prim d (Write 2 (snd p));
+        _ <- Prim d (Write 0 block0);
+        Ret tt.
+
+    Definition ap_op_impl T (op: AtomicPair.Op T) : prog T :=
+      match op with
+      | Get => get
+      | Put p => put p
+      end.
+
+    Definition init : prog InitResult :=
+      len <- Prim d (DiskSize);
+      if len == 5 then
+        _ <- Prim d (Write 0 block0);
+        Ret Initialized
+      else
+        Ret InitFailed.
+
+    Definition impl : InterfaceImpl AtomicPair.Op :=
+      {| op_impl := ap_op_impl;
+         recover_impl := Ret tt;
+         init_impl := then_init (iInit d) init; |}.
+
+    Definition atomic_pair_abstraction (ds : OneDisk.State) (ps : AtomicPair.State) : Prop :=
+      size ds = 5 /\
+      (ds 0 = Some block0 /\ ds 1 = Some (fst ps) /\ ds 2 = Some (snd ps) \/
+       ds 0 = Some block1 /\ ds 3 = Some (fst ps) /\ ds 4 = Some (snd ps)).
+
+    Definition abstr : Abstraction AtomicPair.State :=
+      abstraction_compose
+        (interface_abs d)
+        {| abstraction := atomic_pair_abstraction |}.
+
+    Definition ap : Interface AtomicPair.API.
+      unshelve econstructor.
+      - exact impl.
+      - exact abstr.
+      - destruct op.
+
+        + lift_world.
+          prog_spec_symbolic_execute inv_step.
+
+          all: pose block0_block1_differ.
+          all: unfold atomic_pair_abstraction in *; intuition auto.
+          all: try solve [ exfalso; eapply disk_inbounds_not_none; eauto; omega ].
+          all: try congruence.
+
+          * solve_final_state.
+
+            destruct s; simpl in *; congruence.
+            intuition congruence.
+
+          * solve_final_state.
+
+            destruct s; simpl in *; congruence.
+            intuition congruence.
+
+        + lift_world.
+          prog_spec_symbolic_execute inv_step.
+
+          all: pose block0_block1_differ.
+          all: unfold atomic_pair_abstraction in *; intuition auto.
+          all: try congruence.
+
+          * solve_final_state.
+            repeat autorewrite with upd.
+            repeat ( ( rewrite diskUpd_eq by ( repeat rewrite diskUpd_size; omega ) ) ||
+                     rewrite diskUpd_neq by congruence ).
+            intuition auto.
+
+          * solve_final_state.
+            repeat autorewrite with upd.
+            repeat ( ( rewrite diskUpd_eq by ( repeat rewrite diskUpd_size; omega ) ) ||
+                     rewrite diskUpd_neq by congruence ).
+            intuition auto.
+
+      - cannot_crash.
+      - eapply then_init_compose; eauto.
+        prog_spec_symbolic_execute inv_step.
+
+        + case_eq (state' 1); intros; [ | exfalso ].
+          case_eq (state' 2); intros; [ | exfalso ].
+
+          solve_final_state.
+          autorewrite with upd; auto.
+          repeat ( ( rewrite diskUpd_eq by ( repeat rewrite diskUpd_size; omega ) ) ||
+                   rewrite diskUpd_neq by congruence ).
+          instantiate (1 := (b, b0)).
+          intuition auto.
+
+          eapply disk_inbounds_not_none; eauto; omega.
+          eapply disk_inbounds_not_none; eauto; omega.
+
+        + match_abstraction_for_step; auto.
+
+      Grab Existential Variables.
+      all: eauto.
+
+    Defined.
+
+  End Implementation.
+
+End AtomicPair.
+
+Print Assumptions AtomicPair.ap.
